theories/OGS/Obs.v
@@ -1,10 +1,8 @@
-From Coinduction Require Import coinduction tactics.
-
 From OGS Require Import Prelude.
 From OGS.Utils Require Import Rel.
 From OGS.Ctx Require Import All.
 From OGS.OGS Require Import Subst.
-From OGS.ITree Require Import Event ITree Delay Eq.
+From OGS.ITree Require Import Event ITree Delay Eq Properties.
 
 Open Scope ctx_scope.
 Reserved Notation "O ∙" (at level 5).
@@ -26,43 +24,38 @@ of the language:
 - a map [dom] mapping observations to values filling their copattern
 
 |*)
-#[global] Notation obs_struct T := (f_slice T).
-#[global] Notation dom := s_dom.
-#[global] Coercion s_op : obs_struct >-> Funclass.
-
-Definition pointed_obs {T} (O : obs_struct T) : Fam T := var ∥ ⦇ O ⦈.
+#[global] Notation obs_struct T C := (Oper T C).
+#[global] Notation dom := o_dom.
+Definition pointed_obs `{CC : context T C} (O : Oper T C) : Fam₀ T C
+  := c_var ∥ ⦉O⦊.
 #[global] Notation "O ∙" := (pointed_obs O).
-Definition nf {T} (O : obs_struct T) (X : Fam₁ T) : Fam T := var ∥ (O # X).
+Definition nf `{CC : context T C} (O : obs_struct T C) (X : Fam₁ T C) : Fam₀ T C
+  := c_var ∥ (O # X).
 
-Definition mk_nf {T} {O : obs_struct T} {X : Fam₁ T} {Γ t}
-           (i : t ∈ Γ) (o : O t) (a : dom o =[X]> Γ)
-  : nf O X Γ
-  := ⟨ i | OFill o a ⟩.
-#[global] Notation "i ⋅ o ⦉ a ⦊" := (mk_nf i o a%asgn).
-
-Definition nf_to_obs {T O} {X : Fam₁ T} : forall Γ, nf O X Γ -> O∙ Γ
+Definition nf_to_obs `{CC : context T C} {O} {X : Fam₁ T C} : forall Γ, nf O X Γ -> O∙ Γ
   := f_cut_map f_id₁ forget_args.
 #[global] Coercion nf_to_obs : nf >-> pointed_obs.
 
-Definition then_to_obs {T O} {X : Fam₁ T} {Γ} : delay (nf O X Γ) -> delay (O∙ Γ)
+Definition then_to_obs `{CC : context T C} {O} {X : Fam₁ T C} {Γ}
+  : delay (nf O X Γ) -> delay (O∙ Γ)
   := fmap_delay (nf_to_obs Γ).
 
 Section with_param.
-  Context {T : Type} {O : obs_struct T} {X : Fam₁ T}.
+  Context `{CC : context T C} {O : obs_struct T C} {X : Fam₁ T C}.
 
   Definition nf_ty {Γ} (n : nf O X Γ) : T
     := n.(cut_ty).
-  Definition nf_var {Γ} (n : nf O X Γ) : nf_ty n ∈ Γ
+  Definition nf_var {Γ} (n : nf O X Γ) : Γ ∋ nf_ty n
     := n.(cut_l).
   Definition nf_obs {Γ} (n : nf O X Γ) : O (nf_ty n)
     := n.(cut_r).(fill_op).
-  Definition nf_dom {Γ} (n : nf O X Γ) : ctx T
+  Definition nf_dom {Γ} (n : nf O X Γ) : C
     := dom n.(cut_r).(fill_op).
   Definition nf_args {Γ} (n : nf O X Γ) : nf_dom n =[X]> Γ
     := n.(cut_r).(fill_args).
 
   Variant nf_eq {Γ} : nf O X Γ -> nf O X Γ -> Prop :=
-  | NfEq {t} {i : t ∈ Γ} {o a1 a2} : a1 ≡ₐ a2 -> nf_eq (i⋅o⦉a1⦊) (i⋅o⦉a2⦊).
+  | NfEq {t} {i : Γ ∋ t} {o a1 a2} : a1 ≡ₐ a2 -> nf_eq ⟨i|o⦇a1⦈⟩ ⟨i|o⦇a2⦈⟩.
 
   #[global] Instance nf_eq_Equivalence {Γ} : Equivalence (@nf_eq Γ).
   Proof.
@@ -79,13 +72,9 @@ Section with_param.
   #[global] Instance then_to_obs_proper {Γ}
     : Proper (@comp_eq Γ ==> it_eq (eqᵢ _) (i:=_)) then_to_obs.
   Proof.
-    intros a b; revert a b; unfold it_eq; coinduction R CIH; intros a b H.
-    unfold comp_eq in H; apply it_eq_step in H.
-    cbn in *; unfold observe in H.
-    destruct (_observe a), (_observe b); dependent elimination H; econstructor.
-    - cbn in r_rel; now destruct r_rel.
-    - now apply CIH.
-    - destruct q1.
+    intros a b; unfold comp_eq, then_to_obs, fmap_delay; cbn; intros H.
+    eapply fmap_eq; [ | exact H ].
+    now intros [] ?? [].
   Qed.
 End with_param.
 
